@prefix : <http://open-multinet.info/ontology/omn-domain-wireless#> .
@prefix omn: <http://open-multinet.info/ontology/omn#> .
@prefix owl: <http://www.w3.org/2002/07/owl#> .
@prefix rdf: <http://www.w3.org/1999/02/22-rdf-syntax-ns#> .
@prefix xml: <http://www.w3.org/XML/1998/namespace#> .
@prefix xsd: <http://www.w3.org/2001/XMLSchema#> .
@prefix geni: <http://geni.net/ontology#> .
@prefix rdfs: <http://www.w3.org/2000/01/rdf-schema#> .
@prefix time: <http://www.w3.org/2006/time#> .
@prefix omn_resource: <http://open-multinet.info/ontology/omn-resource#> .
@prefix omn_component: <http://open-multinet.info/ontology/omn-component#> .
@prefix omn_lifecycle: <http://open-multinet.info/ontology/omn-lifecycle#> .
@prefix omn_monitoring: <http://open-multinet.info/ontology/omn-monitoring#> .
@prefix omn_monitoring_unit: <http://open-multinet.info/ontology/omn-monitoring-unit#> .

<http://open-multinet.info/ontology/omn_wireless.owl> a owl:Ontology ;
	rdfs:comment " \"This ontology reuses several concepts from IMINDS wireless ontology\" " .
# 
# 
# #################################################################
# #
# #    Object Properties
# #
# #################################################################
# 
# 
# http://open-multinet.info/ontology/omn#hasComponent

omn:hasComponent a owl:ObjectProperty .
# 
# http://open-multinet.info/ontology/omn#hasReservation

omn:hasReservation a owl:ObjectProperty .
# 
# http://open-multinet.info/ontology/omn-domain-wireless#feature

:feature a owl:ObjectProperty ;
	rdfs:comment "same as http://geni-orca.renci.org/owl/compute.owl#feature" .
# 
# http://open-multinet.info/ontology/omn-domain-wireless#hasAntenna

:hasAntenna a owl:ObjectProperty ;
	rdfs:subPropertyOf :feature ;
	rdfs:domain :WirelessInterface ;
	rdfs:range :Antenna ;
	rdfs:comment "same as http://geni-orca.renci.org/owl/wireless.owl#hasAntenna" .
# 
# http://open-multinet.info/ontology/omn-domain-wireless#hasAntennaBandSupport

:hasAntennaBandSupport a owl:ObjectProperty ;
	rdfs:subPropertyOf :feature ;
	rdfs:range :AntennaBandSupport ;
	rdfs:comment "same as http://geni-orca.renci.org/owl/wireless.owl#hasAntennaBandSupport" .
# 
# http://open-multinet.info/ontology/omn-domain-wireless#hasInputInterface

:hasInputInterface a owl:ObjectProperty ;
	rdfs:subPropertyOf omn_resource:hasInterface ;
	owl:inverseOf :hasOutputInterface ;
	rdfs:comment "same as http://geni-orca.renci.org/owl/compute.owl#hasInputInterface " .
# 
# http://open-multinet.info/ontology/omn-domain-wireless#hasMicroController

:hasMicroController a owl:ObjectProperty ;
	rdfs:subPropertyOf :feature ;
	rdfs:range :MicroController ;
	rdfs:comment "same as http://geni-orca.renci.org/owl/wireless.owl#hasMicroController " .
# 
# http://open-multinet.info/ontology/omn-domain-wireless#hasOutputInterface

:hasOutputInterface a owl:ObjectProperty ;
	rdfs:subPropertyOf omn_resource:hasInterface ;
	rdfs:comment "new property added" .
# 
# http://open-multinet.info/ontology/omn-domain-wireless#hasSensor

:hasSensor a owl:ObjectProperty ;
	rdfs:subPropertyOf :feature ;
	rdfs:comment "same as http://geni-orca.renci.org/owl/wireless.owl#hasSensor " .
# 
# http://open-multinet.info/ontology/omn-domain-wireless#hasSensorModule

:hasSensorModule a owl:ObjectProperty ;
	rdfs:subPropertyOf :feature ;
	rdfs:range :SensorModule ;
	rdfs:comment "same as http://geni-orca.renci.org/owl/wireless.owl#hasSensorModule " .
# 
# http://open-multinet.info/ontology/omn-domain-wireless#isAntennaType

:isAntennaType a owl:ObjectProperty ;
	rdfs:subPropertyOf :feature ;
	rdfs:range :AntennaType ;
	rdfs:comment "same as http://geni-orca.renci.org/owl/wireless.owl#isAntennaType " .
# 
# http://open-multinet.info/ontology/omn-domain-wireless#supportsStandard

:supportsStandard a owl:ObjectProperty ;
	rdfs:subPropertyOf :feature ;
	rdfs:range :Standard ;
	rdfs:comment "new property: taken by old iminds wireless version" .
# 
# http://open-multinet.info/ontology/omn-domain-wireless#usesFrequency

:usesFrequency a owl:ObjectProperty ;
	rdfs:subPropertyOf :feature ;
	rdfs:range :Frequency ;
	rdfs:comment "same as http://geni-orca.renci.org/owl/wireless.owl#usesFrequency" .
# 
# http://open-multinet.info/ontology/omn-monitoring#hasUnit

omn_monitoring:hasUnit a owl:ObjectProperty .
# 
# http://open-multinet.info/ontology/omn-resource#hasInterface

omn_resource:hasInterface a owl:ObjectProperty ;
	rdfs:comment """same as : http://open-multinet.info/ontology/omn-resource#hasInterface
""" .
# 
# 
# 
# #################################################################
# #
# #    Data properties
# #
# #################################################################
# 
# 
# http://open-multinet.info/ontology/omn-domain-wireless#antennaCount

:antennaCount a owl:DatatypeProperty ;
	rdfs:range xsd:integer ;
	rdfs:comment "same as http://geni-orca.renci.org/owl/wireless.owl#antennaCount" .
# 
# http://open-multinet.info/ontology/omn-domain-wireless#antenuation

:antenuation a owl:DatatypeProperty ;
	rdfs:range xsd:double ;
	rdfs:comment "same as http://geni-orca.renci.org/owl/wireless.owl#antenuation" .
# 
# http://open-multinet.info/ontology/omn-domain-wireless#channelNum

:channelNum a owl:DatatypeProperty ;
	rdfs:domain :Channel ;
	rdfs:range xsd:integer ;
	rdfs:comment "new property added" ;
	rdfs:label "Channel Number" .
# 
# http://open-multinet.info/ontology/omn-domain-wireless#lowerBoundFrequency

:lowerBoundFrequency a owl:DatatypeProperty ;
	rdfs:domain :Frequency ;
	rdfs:range xsd:integer .
# 
# http://open-multinet.info/ontology/omn-domain-wireless#upperBoundFrequency

:upperBoundFrequency a owl:DatatypeProperty ;
	rdfs:domain :Frequency ;
	rdfs:range xsd:integer .
# 
# http://open-multinet.info/ontology/omn-domain-wireless#x

:x a owl:DatatypeProperty ;
	rdfs:domain :Location ;
	rdfs:range xsd:integer .
# 
# http://open-multinet.info/ontology/omn-domain-wireless#y

:y a owl:DatatypeProperty ;
	rdfs:domain :Location ;
	rdfs:range xsd:integer .
# 
# http://open-multinet.info/ontology/omn-domain-wireless#z

:z a owl:DatatypeProperty ;
	rdfs:domain :Location ;
	rdfs:range xsd:integer .
# 
# http://open-multinet.info/ontology/omn-lifecycle#hasID

omn_lifecycle:hasID a owl:DatatypeProperty .
# 
# http://open-multinet.info/ontology/omn-monitoring-unit#base

omn_monitoring_unit:base a owl:DatatypeProperty .
# 
# http://open-multinet.info/ontology/omn-monitoring-unit#exponent

omn_monitoring_unit:exponent a owl:DatatypeProperty .
# 
# http://open-multinet.info/ontology/omn-monitoring-unit#symbol

omn_monitoring_unit:symbol a owl:DatatypeProperty .
# 
# 
# 
# #################################################################
# #
# #    Classes
# #
# #################################################################
# 
# 
# http://open-multinet.info/ontology/omn#Component

omn:Component a owl:Class .
# 
# http://open-multinet.info/ontology/omn-domain-wireless#Antenna

:Antenna a owl:Class ;
	rdfs:subClassOf :Feature ;
	rdfs:comment "same as http://geni-orca.renci.org/owl/wireless.owl#Antenna " .
# 
# http://open-multinet.info/ontology/omn-domain-wireless#AntennaBandSupport

:AntennaBandSupport a owl:Class ;
	rdfs:subClassOf :Feature ;
	rdfs:comment "same as http://geni-orca.renci.org/owl/wireless.owl#AntennaBandSupport " .
# 
# http://open-multinet.info/ontology/omn-domain-wireless#AntennaType

:AntennaType a owl:Class ;
	rdfs:subClassOf :Feature ;
	rdfs:comment "same as http://geni-orca.renci.org/owl/wireless.owl#AntennaType " .
# 
# http://open-multinet.info/ontology/omn-domain-wireless#Channel

:Channel a owl:Class ;
	rdfs:subClassOf omn:Component ;
	rdfs:comment "new class added" .
# 
# http://open-multinet.info/ontology/omn-domain-wireless#Feature

:Feature a owl:Class ;
	rdfs:comment "same as  http://geni-orca.renci.org/owl/compute.owl#Feature " .
# 
# http://open-multinet.info/ontology/omn-domain-wireless#Frequency

:Frequency a owl:Class ;
	rdfs:subClassOf :Feature ;
	rdfs:comment "same as http://geni-orca.renci.org/owl/wireless.owl#Frequency " .
# 
# http://open-multinet.info/ontology/omn-domain-wireless#Location

:Location a owl:Class .
# 
# http://open-multinet.info/ontology/omn-domain-wireless#MicroController

:MicroController a owl:Class ;
	rdfs:subClassOf omn:Component .
# 
# http://open-multinet.info/ontology/omn-domain-wireless#Sensor

:Sensor a owl:Class ;
	rdfs:subClassOf omn:Component ;
	rdfs:comment "same as http://geni-orca.renci.org/owl/wireless.owl#Sensor " .
# 
# http://open-multinet.info/ontology/omn-domain-wireless#SensorModule

:SensorModule a owl:Class ;
	rdfs:subClassOf omn:Component ;
	rdfs:comment "same as http://geni-orca.renci.org/owl/wireless.owl#SensorModule " .
# 
# http://open-multinet.info/ontology/omn-domain-wireless#Standard

:Standard a owl:Class ;
	owl:equivalentClass _:genid1 .

_:genid1 a owl:Class ;
	owl:oneOf _:genid5 .

_:genid5 a rdf:List ;
	rdf:first <http://open-multinet.info/ontology/omn_wireless.owl#802.11a> ;
	rdf:rest _:genid4 .

_:genid4 a rdf:List ;
	rdf:first <http://open-multinet.info/ontology/omn_wireless.owl#802.11b> ;
	rdf:rest _:genid3 .

_:genid3 a rdf:List ;
	rdf:first <http://open-multinet.info/ontology/omn_wireless.owl#802.11g> ;
	rdf:rest _:genid2 .

_:genid2 a rdf:List ;
	rdf:first <http://open-multinet.info/ontology/omn_wireless.owl#802.11n> ;
	rdf:rest rdf:nil .

:Standard rdfs:subClassOf :Feature ;
	rdfs:comment "same as http://geni-orca.renci.org/owl/wireless.owl#Standard" .
# 
# http://open-multinet.info/ontology/omn-domain-wireless#WiredInterface

:WiredInterface a owl:Class ;
	rdfs:subClassOf omn_resource:Interface ;
	owl:disjointWith :WirelessInterface ;
	rdfs:comment "same as http://geni-orca.renci.org/owl/compute.owl#WiredInterface " .
# 
# http://open-multinet.info/ontology/omn-domain-wireless#WirelessInterface

:WirelessInterface a owl:Class ;
	rdfs:subClassOf omn_resource:Interface ;
	rdfs:comment "same as http://geni-orca.renci.org/owl/compute.owl#WirelessInterface" .
# 
# http://open-multinet.info/ontology/omn-domain-wireless#xyzCartesianCoordinate

:xyzCartesianCoordinate a owl:Class ;
	owl:equivalentClass _:genid6 .

_:genid6 owl:intersectionOf _:genid11 .

_:genid11 a rdf:List ;
	rdf:first _:genid12 .

_:genid12 a owl:Restriction ;
	owl:onProperty :x ;
	owl:qualifiedCardinality "1"^^xsd:nonNegativeInteger ;
	owl:onDataRange xsd:integer .

_:genid11 rdf:rest _:genid9 .

_:genid9 a rdf:List ;
	rdf:first _:genid10 .

_:genid10 a owl:Restriction ;
	owl:onProperty :y ;
	owl:qualifiedCardinality "1"^^xsd:nonNegativeInteger ;
	owl:onDataRange xsd:integer .

_:genid9 rdf:rest _:genid7 .

_:genid7 a rdf:List ;
	rdf:first _:genid8 .

_:genid8 a owl:Restriction ;
	owl:onProperty :z ;
	owl:qualifiedCardinality "1"^^xsd:nonNegativeInteger ;
	owl:onDataRange xsd:integer .

_:genid7 rdf:rest rdf:nil .

_:genid6 a owl:Class .

:xyzCartesianCoordinate rdfs:subClassOf :Location .
# 
# http://open-multinet.info/ontology/omn-monitoring-unit#DecimalPrefix

omn_monitoring_unit:DecimalPrefix a owl:Class .
# 
# http://open-multinet.info/ontology/omn-resource#Interface

omn_resource:Interface a owl:Class .
# 
# 
# 
# #################################################################
# #
# #    Individuals
# #
# #################################################################
# 
# 
# http://open-multinet.info/ontology/omn-domain-wireless#centimetre

:centimetre a owl:NamedIndividual , omn_monitoring_unit:DecimalPrefix ;
	omn_monitoring_unit:base "10"^^xsd:integer ;
	omn_monitoring_unit:exponent "-3"^^xsd:integer ;
	omn_monitoring_unit:symbol "cm" .
# 
# http://open-multinet.info/ontology/omn-domain-wireless#lowerBoundFrequency

:lowerBoundFrequency a owl:NamedIndividual ;
	omn_monitoring:hasUnit omn_monitoring_unit:persecond .
# 
# http://open-multinet.info/ontology/omn-domain-wireless#upperBoundFrequency

:upperBoundFrequency a owl:NamedIndividual ;
	omn_monitoring:hasUnit omn_monitoring_unit:persecond .
# 
# http://open-multinet.info/ontology/omn-domain-wireless#x

:x a owl:NamedIndividual ;
	omn_monitoring:hasUnit <http://www.w3.org/2002/07/@omn_wireless;centimetre> .
# 
# http://open-multinet.info/ontology/omn-domain-wireless#y

:y a owl:NamedIndividual ;
	omn_monitoring:hasUnit <http://www.w3.org/2002/07/@omn_wireless;centimetre> .
# 
# http://open-multinet.info/ontology/omn-domain-wireless#z

:z a owl:NamedIndividual ;
	omn_monitoring:hasUnit <http://www.w3.org/2002/07/@omn_wireless;centimetre> .
# 
# http://open-multinet.info/ontology/omn-monitoring-unit#persecond

omn_monitoring_unit:persecond a owl:NamedIndividual .
# 
# http://open-multinet.info/ontology/omn_wireless.owl#2.412GHZ

<http://open-multinet.info/ontology/omn_wireless.owl#2.412GHZ> a owl:NamedIndividual , :Frequency ;
	:lowerBoundFrequency "2401000"^^xsd:integer ;
	:upperBoundFrequency "2423000"^^xsd:integer .
# 
# http://open-multinet.info/ontology/omn_wireless.owl#2.417GHZ

<http://open-multinet.info/ontology/omn_wireless.owl#2.417GHZ> a owl:NamedIndividual , :Frequency ;
	:lowerBoundFrequency "2406000"^^xsd:integer ;
	:upperBoundFrequency "2428000"^^xsd:integer .
# 
# http://open-multinet.info/ontology/omn_wireless.owl#802.11a

<http://open-multinet.info/ontology/omn_wireless.owl#802.11a> a owl:NamedIndividual , :Standard ;
	rdfs:comment "same as http://geni-orca.renci.org/owl/wireless.owl#802.11a " ;
	rdfs:label "802.11a" .
# 
# http://open-multinet.info/ontology/omn_wireless.owl#802.11b

<http://open-multinet.info/ontology/omn_wireless.owl#802.11b> a owl:NamedIndividual , :Standard ;
	rdfs:comment "same as http://geni-orca.renci.org/owl/wireless.owl#802.11b " ;
	rdfs:label "802.11b" .
# 
# http://open-multinet.info/ontology/omn_wireless.owl#802.11g

<http://open-multinet.info/ontology/omn_wireless.owl#802.11g> a owl:NamedIndividual , :Standard ;
	rdfs:comment "same as http://geni-orca.renci.org/owl/wireless.owl#802.11g " ;
	rdfs:label "802.11g" .
# 
# http://open-multinet.info/ontology/omn_wireless.owl#802.11n

<http://open-multinet.info/ontology/omn_wireless.owl#802.11n> a owl:NamedIndividual , :Standard ;
	rdfs:comment "same as http://geni-orca.renci.org/owl/wireless.owl#802.11n " ;
	rdfs:label "802.11n" .
# 
# http://www.w3.org/2002/07/@omn_wireless;centimetre

<http://www.w3.org/2002/07/@omn_wireless;centimetre> a owl:NamedIndividual .
# 
# 
# 
# #################################################################
# #
# #    Annotations
# #
# #################################################################
# 
# 

:lowerBoundFrequency rdfs:comment "same as http://geni-orca.renci.org/owl/wireless.owl#lowerBoundFrequency " .
# 

:upperBoundFrequency rdfs:comment "same as http://geni-orca.renci.org/owl/wireless.owl#upperBoundFrequency" .
# 

:x rdfs:comment "same as http://iminds.be/owl/wilab.owl#x" .
# 

:y rdfs:comment "same as http://iminds.be/owl/wilab.owl#y" .
# 

:z rdfs:comment "same as http://iminds.be/owl/wilab.owl#z" .
# 
# 
# 
# #################################################################
# #
# #    General axioms
# #
# #################################################################
# 
# 

_:genid13 a owl:AllDifferent ;
	owl:distinctMembers _:genid17 .

_:genid17 a rdf:List ;
	rdf:first <http://open-multinet.info/ontology/omn_wireless.owl#802.11a> ;
	rdf:rest _:genid16 .

_:genid16 a rdf:List ;
	rdf:first <http://open-multinet.info/ontology/omn_wireless.owl#802.11b> ;
	rdf:rest _:genid15 .

_:genid15 a rdf:List ;
	rdf:first <http://open-multinet.info/ontology/omn_wireless.owl#802.11g> ;
	rdf:rest _:genid14 .

_:genid14 a rdf:List ;
	rdf:first <http://open-multinet.info/ontology/omn_wireless.owl#802.11n> ;
	rdf:rest rdf:nil .
# 
# Generated by the OWL API (version 4.2.8.20170104-2310) https://github.com/owlcs/owlapi
